substitutions combined with mmap

gen-syntax/MMap.v
@@ -1,15 +1,15 @@
-Require Import lib Size.
+Require Import ssrfun lib Size.
 
 Class MMap (A B: Type) := mmap : (A -> A) -> B -> B.
 
 Class MMapLemmas `(mmap : MMap) := {
   mmap_id : mmap id = id;
-  mmap_comp x f g: mmap f (mmap g x) = mmap (fun y => f(g y)) x
+  mmap_comp x f g: mmap f (mmap g x) = mmap (f \o g) x
 }.
 
 Ltac gen_MMap :=
 hnf; match goal with [ |- (?A -> ?A) -> ?B -> ?B] =>
- intros f; fix mmap' 1; intros s;
+intros f; fix mmap' 1; intros s;
 destruct s eqn:E;
 let term := type of s in
 match goal with 
@@ -22,6 +22,7 @@ match goal with
              let s2' := match s2_T with 
                          | A => constr:(f s2) 
                          | B => constr:(mmap' s2)
+                         | bind B => constr:(mmap' s2)
                          | context[B] => constr:(mmap mmap' s2)
                          | context[A] => constr:(mmap f s2)
                          | _ => s2  
@@ -37,22 +38,12 @@ Ltac gen_MMapLemmas :=
 constructor;[
 f_ext; induction 0; simpl; now autorew |
 let x := fresh "x" in intros x; induction x; intros; simpl; now autorew].
-
-Ltac msimpl := 
-  unfold mmap;
-  simpl; 
-  repeat
-match goal with [|- context[?s]] => 
-           match s with 
-             | ?s1 _ _ => match s1 with @mmap _ _ _ => fail 1 | _ => progress change s1 with (@mmap _ _ s1) end
-             | ?s1 _ => match s1 with @mmap _ _ _ => fail 1 | _ => progress change s1 with (@mmap _ _ s1) end
-           end 
-         end.
-
+(*
 Instance mmap_refl (A : Type) : MMap A A := id.
+Arguments mmap_refl _ {_} f /.
 Instance mmap_lemmas_refl (A : Type) : MMapLemmas (mmap_refl A).
 constructor; intuition. Qed.
-
+*)
 Instance mmap_trans (A B C : Type) (mmap1 : MMap A B) (mmap2 : MMap B C) : MMap A C := (fun f => mmap (mmap f)).
 Arguments mmap_trans _ _ _ _ _ _ _ /.
 Instance mmap_lemmas_trans
@@ -60,15 +51,52 @@ Instance mmap_lemmas_trans
 (l1 : MMapLemmas mmap1) (l2 : MMapLemmas mmap2) : MMapLemmas (mmap_trans A B C mmap1 mmap2).
 destruct l1. destruct l2. constructor; cbv; unfold id in *; intros; autorew.
 - now trivial.
-- f_equal. f_ext. intros. now autorew.
+- f_equal. f_ext. intros. unfold funcomp. now autorew.
 Qed.
+
+Hint Rewrite @mmap_id @mmap_comp : mmap.
+
+Ltac msimpl' := 
+  unfold mmap;
+  simpl; 
+repeat match goal with [|- appcontext[?s]] => 
+  match s with 
+    | ?s1 _ => let T := typeof s1 in 
+              match T with MMap _ _ => progress change s1 with (@mmap _ _ s1) end
+  end 
+end.
+
+Ltac msimpl := 
+repeat(
+     msimpl';
+     try(autorewrite with mmap; [idtac | now eauto with typeclass_instances ..])
+    ).
+
+Ltac msimpl'H H := 
+  unfold mmap in H;
+  simpl in H; 
+repeat (
+    let T := typeof H in
+    match T with appcontext[?s] => 
+      match s with 
+        | ?s1 _ => let T := typeof s1 in 
+           match T with MMap _ _ => progress change s1 with (@mmap _ _ s1) in H 
+           end
+      end 
+    end).
+
+Ltac msimplH H := 
+repeat(
+     msimpl'H H;
+     try(autorewrite with mmap in H; [idtac | now eauto with typeclass_instances ..])
+    ).
 
 Instance mmap_list (A : Type) : MMap A (list A).
 gen_MMap. Defined.
 
 Instance mmap_lemmas_list (A : Type) : MMapLemmas (mmap_list A).
 gen_MMapLemmas. Defined.
-
+(*
 Inductive foo :=
   Foo (_ : list (list foo)).
 
@@ -78,14 +106,14 @@ Instance mmap_foo : MMap nat foo.
 gen_MMap. Defined.
 Instance mmap_lemmas_foo : MMapLemmas (mmap_foo).
 constructor. 
-- f_ext. intros x. msimpl. sinduction x.
+- f_ext. intros x. msimpl. sind x; destruct x.
   msimpl. f_equal. induction l.
   + reflexivity.
   + repeat msimpl. f_equal. induction a; 
  repeat(msimpl; autorew; intuition (try somega)).
- apply IHl. intros. apply H. somega.
-- intros x. sinduction x. intros.
+ apply IHl. intros. apply IH. somega.
+- intros x. sind x. intros.
   
-Defined.
+Defined.*)
 
 
